nola/iris/ofe.v
@@ -1,0 +1,6 @@
+(** * Utility on OFEs *)
+
+From nola Require Export prelude.
+From iris.algebra Require Import ofe.
+
+Notation "F $o x" := (oFunctor_apply F x) (at level 20, right associativity).
